src/program_proof/tulip/tulip_proof.v
@@ -1,3 +1,3 @@
 (* paxos *)
 From Perennial.program_proof.tulip.paxos.program Require Export
-  paxos_submit paxos_lookup.
+  start paxos_submit paxos_lookup.
